src/QueryStructure/Automation/SearchTerms/InvertedSearchTerms.v
@@ -2,12 +2,13 @@ Require Import
         Coq.Strings.String
         ADTSynthesis.QueryStructure.Specification.Representation.QueryStructureNotations
         ADTSynthesis.QueryStructure.Specification.SearchTerms.ListInclusion
-        ADTSynthesis.QueryStructure.Implementation.DataStructures.BagADT.IndexSearchTerms.
+        ADTSynthesis.QueryStructure.Implementation.DataStructures.BagADT.IndexSearchTerms
+        ADTSynthesis.QueryStructure.Automation.IndexSelection.
 
 (* Instances for building indexes with make simple indexes. *)
 (* Every Kind of index is keyed on an inductive type with a single constructor*)
 Open Scope string.
-Definition InclusionIndex : string := "inclusionIndex".
+Definition InclusionIndex : string := "InclusionIndex".
 
 (* This is our search term type. *)
 Record InvertedSearchTerm
@@ -21,7 +22,7 @@ Global Instance InvertedIndexDenotation
        (heading : Heading)
        (index : @Attributes heading)
        (projection : @Tuple heading -> list string)
-: @IndexDenotation InclusionIndex heading index :=
+: @IndexDenotation "InclusionIndex" heading index :=
   {| DenoteIndex := InvertedSearchTerm heading; (* Pick search term type *)
      MatchIndex search_term item := (* matching function : DenoteIndex -> Tuple heading -> bool *)
        if IncludedIn_dec (IndexSearchTerm search_term) (projection item) then
@@ -29,7 +30,7 @@ Global Instance InvertedIndexDenotation
        else false |}.
 
 (* Extra type class magic for inverted indices. *)
-Hint Extern 10 (@IndexDenotation InclusionIndex ?heading ?index) =>
+Hint Extern 10 (@IndexDenotation "InclusionIndex" ?heading ?index) =>
 let index_domain := eval hnf in (@Domain heading index) in
 match index_domain with
   | list string =>
@@ -38,3 +39,12 @@ match index_domain with
              (fun tup => GetAttribute tup index ))
 end
 : typeclass_instances.
+
+(* Tactic for associating IncludedIn clauses with InclusionIndex-es*)
+Ltac matchInclusion WhereClause k :=
+  match WhereClause with
+    | fun tups => IncludedIn _ (@?C1 tups) =>
+      let attrs1 := TermAttributes C1 in
+      k (map (fun a12 => (InclusionIndex, (fst a12, snd a12)))
+             (attrs1))
+  end.
