examples/ExtensibleIndexes/Messages.v
@@ -1,3 +1,4 @@
+Require Import Coq.Strings.String.
 Require Import ADTSynthesis.QueryStructure.Automation.AutoDB
         ADTSynthesis.QueryStructure.Automation.IndexSelection
         ADTSynthesis.QueryStructure.Specification.SearchTerms.ListInclusion.
@@ -71,7 +72,11 @@ Proof.
 
   start honing QueryStructure.
 
+  GenerateIndexesForAll matchInclusion ltac:(fun l => make simple indexes using l).
+
+(*
   make simple indexes using [[(EqualityIndex, PHONE_NUMBER); (InclusionIndex, MESSAGE)]; [(EqualityIndex, NAME); (UnIndex, NAME)]].
+ *)
 
   plan.
 
